{
 "cells": [
  {
   "cell_type": "raw",
   "metadata": {
    "raw_mimetype": "text/latex"
   },
   "source": [
    "\\documentclass[11pt]{article}\n",
    "\\usepackage{amsmath, amsfonts, amsthm, amssymb}  % Some math symbols\n",
    "\\usepackage{enumerate}\n",
    "\\usepackage{fullpage}\n",
    "\n",
    "\\usepackage[x11names, rgb]{xcolor}\n",
    "\\usepackage{tikz}\n",
    "\\usepackage{graphicx}\n",
    "\\usetikzlibrary{snakes,arrows,shapes}\n",
    "\n",
    "\\usepackage{listings}\n",
    "\n",
    "\\setlength{\\parindent}{0pt}\n",
    "\\setlength{\\parskip}{5pt plus 1pt}\n",
    "\\pagestyle{empty}\n",
    "\n",
    "\\def\\indented#1{\\list{}{}\\item[]}\n",
    "\\let\\indented=\\endlist\n",
    "\n",
    "\\newcounter{questionCounter}\n",
    "\\newenvironment{question}[2][\\arabic{questionCounter}]{%\n",
    "    \\addtocounter{questionCounter}{1}%\n",
    "    \\setcounter{partCounter}{0}%\n",
    "    \\vspace{.25in} \\hrule \\vspace{0.5em}%\n",
    "        \\noindent{\\bf #2}%\n",
    "    \\vspace{0.8em} \\hrule \\vspace{.10in}%\n",
    "}{}\n",
    "\n",
    "\\newcounter{partCounter}[questionCounter]\n",
    "\\renewenvironment{part}[1][\\alph{partCounter}]{%\n",
    "    \\addtocounter{partCounter}{1}%\n",
    "    \\vspace{.10in}%\n",
    "    \\begin{indented}%\n",
    "       {\\bf (#1)} %\n",
    "}{\\end{indented}}\n",
    "\n",
    "%%%%%%%%%%%%%%%%% Identifying Information %%%%%%%%%%%%%%%%%\n",
    "%% This is here, so that you can make your homework look %%\n",
    "%% pretty when you compile it.                           %%\n",
    "%%%%%%%%%%%%%%%%%%%%%%%%%%%%%%%%%%%%%%%%%%%%%%%%%%%%%%%%%%%\n",
    "\\newcommand{\\myname}{Akshay Chalana}\n",
    "\\newcommand{\\myemail}{ac2zoom@cs.uw.edu}\n",
    "\\newcommand{\\myhwname}{Math 336: Homework 1}\n",
    "%%%%%%%%%%%%%%%%%%%%%%%%%%%%%%%%%%%%%%%%%%%%%%%%%%%%%%%%%%%\n",
    "\\begin{document}\n",
    "\\begin{center}\n",
    "    {\\Large \\myhwname} \\\\\n",
    "    \\myname \\\\\n",
    "    \\myemail \\\\\n",
    "    \\today\n",
    "\\end{center}\n",
    "\n",
    "\\begin{question}{\\S1.1: 6}\n",
    "    For fixed $a\\in\\mathbb{C}$, show that $|z-a|/|1-\\bar{a}z|=1$ if $|z|=1$ and $1-\\bar{a}z\\neq0$. \\\\\\\\\n",
    "    This is to say that, for fixed $a\\in\\mathbb{C}$, $|z-a|=|1-\\bar{a}z|$.  If $|z|=|\\bar{z}|=1$, $|z-a|=|z-a||\\bar{z}|=|z\\bar{z}-a\\bar{z}|=|1-a\\bar{z}|=|1-\\bar{a}z|$, which demonstrates this equality. If the denominator above ($|1-\\bar{a}z|$) is 0, the value of the quotient is undefined, so we must state this condition as well.\n",
    "\\end{question}\n",
    "\\begin{question}{\\S1.1: 7}\n",
    "    Fix $\\rho>0$, $\\rho\\neq1$, and fix $z_0,z_1\\in\\mathbb{C}$. Show that the set of $z$ satisfying $|z-z_0|=\\rho|z-z_1|$ is a circle. Sketch it for $\\rho=\\frac{1}{2}$ and $\\rho=2$, with $z_0=0$ and $z_1=1$. What happens when $\\rho=1$? \\\\\\\\\n",
    "    First note that the equation of the circle centered at $(a,b)$ is $(x-a)^2+(y-b)^2=r^2$. \\\\\n",
    "    Starting with $|z-z_0|=\\rho|z-z_1|$, we can get $|z-z_0|^2=\\rho^2|z-z_1|^2$. \\\\\n",
    "    Let $z=x+iy$, $z_0=x_0+iy_0$, and $z_1=x_1+iy_1$.  We thus have $(x-x_0)^2+(y-y_0)^2=\\rho^2((x-x_1)^2+(y-y_0)^2)$. This is equivalent to:\n",
    "    $$(1-\\rho^2)x^2-2(x_0-\\rho^2x_1)x+(x_0^2-\\rho^2x_1^2)+(1-\\rho^2)y^2-2(y_0-\\rho^2y_1)y+(y_0^2-\\rho^2y_1^2)=0$$\n",
    "    $$x^2-2\\frac{(x_0-\\rho^2x_1)}{1-\\rho^2}x+\\frac{(x_0^2-\\rho^2x_1^2)}{1-\\rho^2}+y^2-2\\frac{(y_0-\\rho^2y_1)}{1-\\rho^2}y+\\frac{(y_0^2-\\rho^2y_1^2)}{1-\\rho^2}=0$$\n",
    "    $$(x-\\frac{x_0-\\rho^2x_1}{1-\\rho^2})^2+\\frac{(1-\\rho^2)(x_0^2-\\rho^2x_1^2)-(x_0-\\rho^2x_1)^2}{(1-\\rho^2)^2}+(y-\\frac{y_0-\\rho^2y_1}{1-\\rho^2})^2+\\frac{(1-\\rho^2)(y_0^2-\\rho^2y_1^2)-(y_0-\\rho^2y_1)^2}{(1-\\rho^2)^2}=0$$\n",
    "    $$(x-\\frac{x_0-\\rho^2x_1}{1-\\rho^2})^2+(y-\\frac{y_0-\\rho^2y_1}{1-\\rho^2})^2=$$\n",
    "    $$\\frac{(x_0-\\rho^2x_1)^2+(y_0-\\rho^2y_1)^2-(1-\\rho^2)(x_0^2+y_0^2-\\rho^2(x_1^2+y_1^2))}{(1-\\rho^2)^2}$$\n",
    "    $$=\\frac{\\rho^2((x_1-x_0)^2+(y_1-y_0)^2)}{(1-\\rho^2)^2}$$\n",
    "    This is the equation for a circle. \\\\\\\\\n",
    "    When $z_0=0$ and $z_1=1$, we have\n",
    "    $$(x-\\frac{-\\rho^2}{1-\\rho^2})^2+y^2=(\\frac{\\rho}{1-\\rho^2})^2$$\n",
    "    At $\\rho=\\frac{1}{2}$, we have a circle centered at $(-\\frac{1}{3},0)$ with radius $\\frac{2}{3}$. When $\\rho=2$, we have a circle of the same radius, but centered at $(\\frac{4}{3},0)$. $\\rho=1$ gives us a direct modfication of our original equation: $|z-z_0|=|z-z_1|$, which is the line $\\textrm{Re}z=\\frac{1}{2}$. \n",
    "\\end{question}\n",
    "\\begin{question}{\\S1.2: 6}\n",
    "    Fix $n\\geq1$. Show that the $n$th roots of unity $\\omega_0,...,\\omega_{n-1}$ satisfy:\n",
    "    \\begin{part}\n",
    "        $(z-\\omega_0)(z-\\omega_1)...(z-\\omega_{n-1})=z^n-1$ \\\\\n",
    "        If each $\\omega_j$ is a root of unity, then $\\omega_j=e^{2\\pi ji/n}$. We know that each $\\omega_j$ is a root of $z^n-1$ because $\\omega_j^n-1=(e^{2\\pi ji/n})^n-1=e^{2\\pi ji}-1=e^{2\\pi ji}-1=0$.  Since the roots are simple and the coefficient of the $z^n$ term is 1, the FTA gives us that $z^n-1=(z-\\omega_0)(z-\\omega_1)...(z-\\omega_{n-1})$.\n",
    "    \\end{part}\n",
    "    \\begin{part}\n",
    "        $\\omega_0+...+\\omega_{n-1})=0$ if $n\\geq2$\\\\\n",
    "        Multiplying the factors of the product from the previous answer, we have\n",
    "        $$z^n-1=z^n-(\\omega_0+\\omega_1+...+w_{n-1})z^{n-1}+c_2z^{n-2}+...+(-1)^n\\omega_0\\omega_1...w_{n-1}$$\n",
    "        By considering coefficients, we see that\n",
    "        $$\\omega_0+\\omega_1+...+\\omega_{n-1}=0$$\n",
    "        if $n\\geq2$.\n",
    "    \\end{part}\n",
    "    \\begin{part}\n",
    "        $\\omega_o...\\omega_{n-1}=(-1)^{n-1}$\\\\\n",
    "        It follows directly from the previous answer that\n",
    "        $$-1=(-1)^n\\omega_0\\omega_1...\\omega_{n-1}\\Leftrightarrow\\omega_0\\omega_1...\\omega_{n-1}=(-1)^{n-1}$$\n",
    "    \\end{part}\n",
    "    \\begin{part}\n",
    "        $\\sum_{j=0}^{n-1}\\omega_j^k=\\begin{array}{cc}\n",
    "  \\{ & \n",
    "    \\begin{array}{cc}\n",
    "      0, & 1\\leq k\\leq n-1 \\    n, & k=n\n",
    "    \\end{array}\n",
    "\\end{array}$\n",
    "        When $1\\leq k\\leq n-1$\n",
    "        $$\\sum_{j=0}^{n-1}\\omega_j^k=\\sum_{j=0}^{n-1}(e^{2\\pi ji/n})^k=\\sum_{j=0}^{n-1}(e^{2\\pi ki/n})^j=\\frac{1-(e^{2\\pi ki/n})^n}{1-e^{2\\pi ki/n}}=\\frac{1-e^{2\\pi ki}}{1-e^{2\\pi ki/n}}=0$$\n",
    "        When $k=n$\n",
    "        $$\\sum_{j=0}^{n-1}\\omega_j^k=\\sum_{j=0}^{n-1}(e^{2\\pi ji/n})^n=\\sum_{j=0}^{n-1}e^{2\\pi ji}=\\sum_{j=0}^{n-1}1=n$$\n",
    "    \\end{part}\n",
    "\\end{question}\n",
    "\\begin{question}{\\S1.2: 7}\n",
    "    \n",
    "\\end{question}\n",
    "\\begin{question}{\\S1.7: 4}\n",
    "    \n",
    "\\end{question}\n",
    "\\begin{question}{\\S1.7: 5}\n",
    "    \n",
    "\\end{question}\n",
    "\\end{document}"
   ]
  },
  {
   "cell_type": "markdown",
   "metadata": {},
   "source": []
  },
  {
   "cell_type": "code",
   "execution_count": null,
   "metadata": {
    "collapsed": true
   },
   "outputs": [],
   "source": []
  }
 ],
 "metadata": {
  "celltoolbar": "Raw Cell Format",
  "kernelspec": {
   "display_name": "Python 3",
   "language": "python",
   "name": "python3"
  },
  "language_info": {
   "codemirror_mode": {
    "name": "ipython",
    "version": 3
   },
   "file_extension": ".py",
   "mimetype": "text/x-python",
   "name": "python",
   "nbconvert_exporter": "python",
   "pygments_lexer": "ipython3",
   "version": "3.5.2"
  }
 },
 "nbformat": 4,
 "nbformat_minor": 2
}
